x86model/Model/ParserArg.v
@@ -53,16 +53,17 @@ Module X86_PARSER_ARG.
   Inductive type : Set := 
   | Int_t : type
   | Register_t : type
-  | Byte_t : type
-  | Half_t : type
-  | Word_t : type
-  | Double_Word_t : type
-  | Ten_Byte_t : type
+  | BitVector_t : nat -> type (* a bit vector of a certain width *)
+  (* | Byte_t : type *)
+  (* | Half_t : type *)
+  (* | Word_t : type *)
+  (* | Double_Word_t : type *)
+  (* | Ten_Byte_t : type *)
   | Scale_t : type
   | Condition_t : type
   | Address_t : type
   | Operand_t : type
-  | Fpu_Register_t : type
+  (* | Fpu_Register_t : type *)
   | Fp_Debug_Register_t : type
   | Fp_Operand_t : type 
   | MMX_Granularity_t : type
@@ -81,25 +82,34 @@ Module X86_PARSER_ARG.
   (* Need pairs at this level if I want to have options of pairs*)
   | UPair_t (t1 t2: type) : type. 
 
+  Definition Byte_t := BitVector_t 7.
+  Definition Half_t := BitVector_t 15.
+  Definition Word_t := BitVector_t 31.
+  Definition Double_Word_t := BitVector_t 63.
+  Definition Ten_Byte_t := BitVector_t 79.
+  Definition Fpu_Register_t := BitVector_t 2.
+
   Definition tipe := type.
   Definition tipe_eq : forall (t1 t2:tipe), {t1=t2} + {t1<>t2}.
     intros ; decide equality.
+    apply eq_nat_dec.
   Defined.
 
   Fixpoint tipe_m (t:tipe) := 
     match t with 
       | Int_t => Z
       | Register_t => register
-      | Byte_t => int8
-      | Half_t => int16
-      | Word_t => int32
-      | Double_Word_t => int64
-      | Ten_Byte_t => int80
+      | BitVector_t n => Word.int n
+      (* | Byte_t => int8 *)
+      (* | Half_t => int16 *)
+      (* | Word_t => int32 *)
+      (* | Double_Word_t => int64 *)
+      (* | Ten_Byte_t => int80 *)
       | Scale_t => scale
       | Condition_t => condition_type
       | Address_t => address
       | Operand_t => operand
-      | Fpu_Register_t => int3
+      (* | Fpu_Register_t => int3 *)
       | Fp_Debug_Register_t => fp_debug_register
       | Fp_Operand_t => fp_operand  
       | MMX_Granularity_t => mmx_granularity
